theories/ordinals/Ackermann/folLogic3.v
@@ -26,7 +26,6 @@ Let var := var L.
 Let apply := apply L.
 Let equal := equal L.
 Let atomic := atomic L.
-Let orH := orH L.
 Let andH := andH L.
 Let existH := existH L.
 Let iffH := iffH L.
